<section xmlns:xi="http://www.w3.org/2001/XInclude" xml:id="s_quotients">
  <title>Quotients</title>
  <introduction>
    <p>

    </p>
</introduction>
<project xml:id="top_eg_quotient_space">
  <title>Quotient space</title>
  <p>
    Let <m>(X,\mathcal{T})</m> be a topological space, <m>\sim</m> an equivalence relation on <m>X</m>, <m>X^*=X/\sim</m> the set of equivalence classes of <m>\sim</m>, and <m>q\colon X\rightarrow X^*</m> the map sending <m>x\in X</m> to its equivalence class <m>[x]_\sim\in X^*</m>. The set
    <me>
      \mathcal{T}_{\operatorname{quot}}=\{U\subset X^*\colon q^{-1}(U)\in \mathcal{T}\}
    </me>
    is a topology on <m>X^*</m> called the <term>quotient topology</term>. The map <m>q\colon X\rightarrow X^*</m> is a <em>quotient map</em>: that is, it is surjective and satisfies <m>V\subseteq X^*</m> is open if and only if <m>q^{-1}(V)</m> is open.
  </p>
  <proof>
    <p>
      That <m>\mathcal{T}_{\operatorname{quot}}</m> is a topology follows easily from properties of preimages of sets; and it satisfies the quotient map properties essentially by definition.
    </p>
  </proof>
</project>
<example xml:id="eg_quotient_no_proof">
  <statement>
    <p>
      For each quotient space description give an explicit description of the equivalence classes and identify (without proof) what familiar space the quotient might be homeomorphic to.
    </p>
    <ol>
      <li>
        <p>
          <m>X=[0,1]</m>, <m>X^*</m> obtained by identifying <m>0</m> and <m>1</m>
        </p>
      </li>
      <li>
        <p>
          <m>X=\R</m>, <m>X^*=X/\sim</m>, where <m>x\sim y</m> if and only if <m>x=y+n</m> for some <m>n\in \Z</m>
        </p>
      </li>
      <li>
        <p>
          <m>X=[0,1]\times [0,1]</m>, <m>X^*</m> obtained by identifying <m>P=(0,y)</m> and <m>Q=(1,y)</m> for all <m>y\in [0,1]</m>
        </p>
      </li>
      <li>
        <p>
          <m>X=[0,1]\times [0,1]</m>, <m>X^*</m> obtained by identifying <m>P=(0,y)</m> and <m>Q=(1,y)</m> for all <m>y\in [0,1]</m> and all <m>R=(x,0)</m> and <m>S=(x,1)</m> for <m>x\in [0,1]</m>.
        </p>
      </li>
    </ol>
  </statement>
  <solution>
    <p>

    </p>
  </solution>
</example>
<definition xml:id="d_quotient_map">
  <statement>
    <p>
      Let <m>X</m> and <m>Y</m> be topological spaces. A function <m>f\colon X\rightarrow Y</m> is a <term>quotient map</term> if it satisfies the following properties:
      <ol>
        <li>
          <p>
            <m>f</m> is surjective;
          </p>
        </li>
        <li>
          <p>
            <m>V\subseteq Y</m> is open if and only if <m>f^{-1}(V)\subseteq X</m> is open.
          </p>
        </li>
      </ol>
      It follows immediately from the definition that a quotient map is continuous.
    </p>
  </statement>
</definition>
<definition xml:id="d_saturated">
  <title>Saturated sets</title>
  <statement>
    <p>
      Let <m>f\colon X\rightarrow Y</m>.
            A set <m>A\subseteq X</m> is saturated with respect to <m>f</m> if <m>f^{-1}(f(A))=A</m>. Equivalently, <m>A</m> is saturated if if whenever <m>x\in A</m> we have <m>f^{-1}(\{f(x)\})\subseteq A</m>.
    </p>
  </statement>
</definition>
<theorem xml:id="th_quotientmap_props">
  <title>Quotient map properties</title>
  <statement>
    <ol>
      <li>
        <p>
          Let <m>f\colon X\rightarrow Y</m> be a continuous surjective function. The following statements are equivalent.
          <ol>
            <li>
              <p>
                <m>f</m> is a quotient map.
              </p>
            </li>
            <li>
              <p>
                <m>f(U)</m> is open for all open saturated sets <m>U\subseteq X</m>.
              </p>
            </li>
            <li>
              <p>
                <m>f(C)</m> is closed for all closed saturated subsets <m>C\subseteq X</m>.
              </p>
            </li>
          </ol>
        </p>
      </li>
      <li>
        <p>
          Let <m>f</m> be continuous and surjective. If <m>f</m> is open or closed, then it is a quotient map.
        </p>
      </li>
      <li>
        <p>
          The composition of two quotient maps is a quotient map.
        </p>
      </li>
    </ol>
  </statement>
  <p>
    Statement (3) is straightforward. Statement (2) follows easily from (1) using equivalent statements (b) and (c), respectively.
  </p>
  <proof>

    <title>Proof of (1)</title>
    <p>
      We prove <m>(a)\iff (b)</m> and <m>(b)\iff (c)</m>.
    </p>
    <p>
      <m>(a)\implies (b)</m>. Assume <m>f</m> is a quotient map. Let <m>U\subseteq X</m> be open and saturated. Since <m>f</m> is a quotient map, to show <m>V=f(U)</m> is open, it is enough to show <m>f^{-1}(V)=f^{-1}(f(U))</m> is open. I claim <m>f^{-1}(f(U))=U</m>, whence the claim follows. In general for any function of sets we have <m>f^{-1}(f(U))\supseteq U</m>. (Check for yourself.) Since <m>U</m> is saturated, the reverse inclusion also holds. Indeed, if <m>x\in f^{-1}(f(U))</m>, then <m>f(x)\in f(U)</m> and thus <m>f(x)=f(u)</m> for some <m>u\in U</m>; since <m>U</m> is saturated, we have <m>x\in U</m>.
    </p>
    <p>
      <m>(b)\implies (a)</m>. Assume <m>U=f^{-1}(V)</m> be open for <m>V\subseteq Y</m>. We wish to show that <m>V</m> is open in <m>Y</m>. First observe that <m>f^{-1}(V)</m> is saturated: if <m>x\in f^{-1}(V)</m>, then <m>f^{-1}(\{f(x)\})\subseteq f^{-1}(V)</m>. Since <m>f</m> satisfies <m>(b)</m> and <m>U</m> is an open saturated set, we have <m>f(U)</m> open. I claim <m>f(U)=f(f^{-1}(V))=V</m>, showing <m>V</m> is open. In general we always have
      <m>f(f^{-1}(V))\subseteq V</m> for any function of sets. For the other inclusion, given <m>y\in V</m>, there is an <m>x\in X</m> such that <m>f(x)=y</m>; then <m>x\in f^{-1}(V)</m> and <m>f(x)=y</m>, showing <m>y\in f(f^{-1}(V))</m>.
    </p>
    <p>
      <m>(b)\implies (c)</m>. Let <m>C</m> be a saturated closed map. First I claim that the open set <m>U=X-C</m> is saturated. To see why, suppose <m>y=f(x)</m> for some <m>x\in U</m>. Since <m>x\notin C</m> and <m>C</m> is saturated, we must have <m>f^{-1}(\{y\})\cap C=\emptyset</m>. Thus <m>f^{-1}(\{y\})\subseteq U</m>, as desired. Next, I claim <m>f(U)=Y-f(C)</m>. We have already seen that if <m>y\in f(U)</m>, then <m>f^{-1}(\{y\})\cap C=\emptyset</m>,
      and hence <m>y\notin f(C)</m>. This proves <m>f(U)\subseteq Y-f(C)</m>. For the other inclusion, given any <m>y\in Y-f(C)</m>, by surjectivity there is some <m>x\in X</m> such that <m>f(x)=y</m>; since <m>y\notin f(C)</m> we must have <m>x\in U</m>; thus <m>y\in f(U)</m>. This proves <m>f(U)=X-f(C)</m>. Since <m>f</m> satisfies (b), <m>f(U)</m> is open. We conclude that <m>f(C)</m> is closed, as desired.
    </p>
    <p>
      <m>(c)\implies (b)</m>. This argument is essentially identical to the one above.
    </p>
  </proof>

</theorem>

<theorem xml:id="th_quotientmap_mappingprop">
  <title>Mapping property of quotient maps</title>
  <statement>
    <p>
      Let <m>p\colon X\rightarrow Y</m> be a quotient map. Given any continuous function <m>g\colon X\rightarrow Z</m> satisfying
      <men xml:id="eq_agree_on_fibers">
        p(x)=p(x') \implies g(x)=g(x')
      </men>
      for all <m>x, x'\in X</m> there is a unique continuous function <m>f\colon Y\rightarrow Z</m> satisfying <m>g=f\circ p</m>.
      <image xml:id="im_quotientmap_pros" width="25%">
      <latex-image>
        \begin{tikzcd}
           X \arrow[rd, "g"] \arrow[d, twoheadrightarrow,"p"']\amp \\
          Y \arrow[r,dotted,"\exists! f"'] \amp Z
        \end{tikzcd}
      </latex-image>
      Furthermore, the function <m>f</m> is a projection map if and only if <m>g</m> is a projection map.
      </image>
    </p>
  </statement>
  <proof>
    <p>
      Assume we have <m>g\colon X\rightarrow Z</m> as described. Define <m>f\colon Y\rightarrow Z</m> via the following recipe: given <m>y\in Y</m>, pick any <m>x\in X</m> such that <m>p(x)=y</m> (possible since <m>p</m> is surjective); now define <m>f(y)=g(x)</m>. Two comments:
      <ol>
        <li>
          <p>
            To make sure <m>f</m> as described is well-defined, we must make sure that the definition of <m>f(y)</m> does not depend on the choice of <m>x</m> involve: <ie />, if you happen to pick another <m>x'</m> such that <m>p(x')=y</m>, we must make sure that <m>g(x)=g(x')</m>. This is precisely what is guaranteed by the condition that <m>p(x)=p(x')\implies g(x)=g(x')</m>.
          </p>
        </li>
        <li>
          <p>
            Since we want <m>g=f\circ p</m>, this definition of <m>f</m> is forced upon us: given <m>y=p(x)</m>, we must have <m>f(y)=f(p(x))=g(x)</m>. Thus <m>f</m> is unique.
          </p>
        </li>
      </ol>
      Now we must show <m>f</m> is continuous. We must show, given any open <m>V\subseteq Z</m> the set <m>U=f^{-1}(V)</m> is open. To do so we use the fact that <m>p</m> is a quotient map: that is, we need only show that <m>p^{-1}(U)</m> is open in <m>X</m>. But we have
      <me>
        p^{-1}(U)=p^{-1}(f^{-1}(V))=(f\circ p)^{-1}(V)=g^{-1}(V),
      </me>
      since <m>g=f\circ p</m>. Since <m>g</m> is continuous, we conclude that <m>p^{-1}(U)=g^{-1}(V)</m> is open, as desired.
    </p>
    <p>
      Lastly, we look at when <m>f</m> is a quotient map. If <m>f</m> is a quotient map, then so is the composition <m>g=f\circ p</m> by statement (3) of <xref ref="th_quotientmap_props"/>. Assume <m>g</m> is a quotient map. Since <m>g</m> is surjective and <m>g=f\circ p</m>, it follows that <m>f</m> must be surjective. Now suppose <m>U=f^{-1}(V)</m> is open in <m>Y</m>. Since <m>p</m> is continuous, <m>p^{-1}(U)</m> is open in <m>X</m>. As we saw above, <m>p^{-1}(U)=g^{-1}(V)</m>, which is a saturated open set of <m>X</m>. Since <m>g</m> is a quotient map, the set <m>g(g^{-1}(V))</m>
       is open. But again, because <m>g</m> is surejective, we have <m>g(g^{-1}(V))=V</m>.
    </p>
  </proof>

</theorem>
<definition xml:id="d_fibers_agree">
  <title>Fibers of maps</title>
  <statement>
    <p>
      For any function <m>f\colon X\rightarrow Y</m> between sets and element <m>y\in Y</m>, we call <m>f^{-1}(\{y\})</m> the <term>fiber of <m>f</m> lying over <m>y</m></term>. We say a function <m>g\colon X\rightarrow Z</m> <term>agrees on fibers</term> of <m>f</m> if
      <me>
        f(x)=f(x')\implies g(x)=g(x')
      </me>.
    </p>
  </statement>
</definition>
<corollary xml:id="cor_quotientspace_props">
  <title>Mapping property of quotients</title>
  <statement>
    <p>
      Let <m>X^*</m> be the quotient space of <m>X</m> by the equivalence relation <m>\sim</m>, and let <m>q\colon X\rightarrow X^*</m> be the corresponding quotient map. Let <m>g\colon X\rightarrow Z</m> be a continuous function that agrees on fibers of <m>q</m> (<ie />, <m>x\sim x'\implies g(x)=g(x')</m>).
      <ol>
        <li>
          <p>
            There is a unique continuous function <m>f</m> satisfying <m>g=f\circ q</m>; and <m>f</m> is a quotient map if and only if <m>g</m> is a quotient map.
            <image xml:id="im_quotientspace_prop" width="25%">
            <latex-image>
              \begin{tikzcd}
                 X \arrow[rd, twoheadrightarrow,"g"] \arrow[d, twoheadrightarrow,"p"']\amp \\
                X^* \arrow[r,dotted,"\exists! f"'] \amp Y
              \end{tikzcd}
            </latex-image>
          </image>
          </p>
        </li>
        <li>
          <p>
            The function <m>f</m> is a homeomorphism if and only if <m>g</m> is a quotient map and satisfies
            <me>
              g(x)=g(x') \iff x\sim x' (\text{equivalently, } g(x)=g(x')\iff q(x)=q(x'))
            </me>
            for all <m>x, x'\in X</m>.
          </p>
        </li>
      </ol>
    </p>
  </statement>
  <proof>
    <ol>
      <li>
        <p>
          The statement is a direct consequence of <xref ref="th_quotientmap_mappingprop"/> by setting <m>Y=X^*</m> and <m>p=q</m>, and understanding that the implication <m>x\sim x'\implies g(x)=g(x')</m> is equivalent to <m>p(x)=p(x')\implies g(x)=g(x')</m>.
        </p>
      </li>
      <li>
        <p>
          The condition <m>x\sim x' \iff g(x)=g(x')</m> guarantees that the function <m>f\colon X^*\rightarrow Y</m> is injective. The condition of <m>g</m> being a quotient map is equivalent to <m>f</m> being a quotient map according to <xref ref="th_quotientmap_mappingprop"/>. Thus the two conditions taken together are equivalent to <m>f</m> being a bijective quotient map. This in turn is equivalent to being a homeomorphism by equivalent statement 1.b of <xref ref="th_continuous_equivalence"/>, since <em>all</em> subsets of <m>X</m> are saturated with respect to an invertible function <m>f</m>.
        </p>
      </li>
    </ol>

  </proof>

</corollary>
<corollary xml:id="cor_quotient_factor">
  <title>Factoring maps through a quotient</title>
  <statement>
    <p>
      Let <m>g\colon X\rightarrow Y</m> be a surjective continuous map, and let <m>X^*</m> be the quotient obtained from <m>X</m> by treating each fiber <m>g^{-1}(\{y\})</m>, <m>y\in Y</m>,  as a single point: <ie />, the equivalence relation is <m>x\sim x'\iff g(x)=g(x')</m>.
    </p>
    <ol>
      <li>
        <p>
          There is a unique bijective continuous function <m>f\colon X^*\rightarrow Y</m> satisfying <m>g=f\circ q</m>.
        </p>
      </li>
      <li>
        <p>
          The function <m>f</m> is a homeomorphism if and only if <m>g</m> is a quotient map.
        </p>
      </li>
      <li>
        <p>
          If <m>Y</m> is Hausdorff, then <m>X^*</m> is Hausdorff.
        </p>
      </li>
    </ol>
  </statement>
  <proof>
    <p>
      With the exception of (3), this corollary follows essentially directly from <xref ref="cor_quotientspace_props"/>. Statement (3) follows directly from (1). In fact, more generally, if <m>f\colon X\rightarrow Y</m> is a bijective continuous map, and <m>Y</m> is Hausdorff, then <m>X</m> is Hausdorff.
    </p>
  </proof>

</corollary>
<!-- <p>
  Lastly, the following result is also helpful when dealing with quotient spaces. I omit the proof, which you can find in Munkres.
</p>
<theorem xml:id="th_quotient_subspace">
  <title>Quotients and subspaces</title>
  <statement>
    <p>
      Let <m>p\colon X\rightarrow Y</m> be a quotient map, and let <m>A\subseteq X</m> be a subspace that is saturated with respect to <m>p</m>. Let <m>q=p\vert_A\colon A\rightarrow p(A)</m> be the restriction of <m>p</m> to <m>A</m>.
    </p>
    <ol>
      <li>
        <p>
          If <m>A</m> is either open or closed, then <m>q</m> is a quotient map.
        </p>
      </li>
      <li>
        <p>
          If <m>p</m> is either an open or a closed map, then <m>q</m> is a quotient map.
        </p>
      </li>
    </ol>
  </statement>
</theorem> -->

<example xml:id="eg_RmodZ">
  <title>The circle as a quotient space</title>
  <statement>
    <p>
      Let <m>X^*</m> denote the quotient obtained from <m>X=[0,1]</m> after identifying <m>0</m> and <m>1</m>, and let <m>\R/\Z</m> denote the quotient of <m>\R</m> by the equivalence relation <m>x\sim y</m> if and only if <m>x=y+n</m> for some <m>n\in Z</m>. Prove that <m>\R/\Z</m> is homeomorphic to <m>S^1=\{(x,y)\colon x^2+y^2=1\}</m>.
    </p>
    <ol>
      <li>
        <p>
          Prove: <m>X^*\cong \R/\Z</m>
        </p>
      </li>
      <li>
        <p>
          Prove: <m>X^*\cong \R/\Z\cong S^1</m>.
        </p>
      </li>
    </ol>
    <p>
      Note: once we have some notions about compactness under our belt it will be easy to show directly that <m>X^*\cong S^1</m>. Part (2) is a workaround for the time being.
    </p>
  </statement>
  <solution>
    <ol>
      <li>
        <p>
          Consider the map <m>g</m> defined by composition
          <image xml:id="eg_quot_g" width="50%">
            <latex-image>
              \begin{tikzcd}
                 {[0,1]} \arrow[r,hookrightarrow,"i"] \arrow[rr, bend right=30, "g"'] \amp \R \arrow[r, twoheadrightarrow,"q"] \amp \R/\Z \\
              \end{tikzcd}
            </latex-image>
          </image>
          where <m>q</m> is the quotient map from <m>\R</m> to <m>\R/\Z</m>.
          It is easy to see that <m>g</m> is surjective and satisfies <m>g(t)=g(t')</m> if and only if <m>t=t'</m> or <m>t,t'\in \{0,1\}</m>. From <xref ref="cor_quotientspace_props"/> we conclude that <m>g</m> gives rise to a bijective continuous function <m>f\colon X^*\rightarrow \R/\Z</m>. Concretely, <m>f</m> takes an equivalence class <m>[t]\in X^*</m> and maps it to the equivalence class <m>\{t+n\colon n\in \Z\}</m> in <m>\R/\Z</m>. Furthermore, to show <m>f</m> is a homeomorphism it is enough to prove that <m>g\colon [0,1]\rightarrow \R/\Z</m>
          is a quotient map. In fact, we can show that <m>g</m> is a closed map. Take a closed set <m>C\subseteq [0,1]</m>. To show its image <m>g(C)</m> is closed in <m>\R/Z</m>, we need only show, using the fact that <m>q</m> is a quotient map, that <m>q^{-1}(g(C))</m> is closed in <m>\R/\Z</m>. We have <m>q^{-1}(g(C))=C+\Z=\{c+n\colon c\in C, n\in \Z\}</m>. This set is the result of starting with our original closed set <m>C\subseteq [0,1]</m> and taking the union of translated copies of the form <m>C+n\subseteq [n,n+1]</m>, where <m>n\in \Z</m>.
          It is easy to see that each translate <m>C+n</m> is closed; since furthermore <m>C+n\subseteq [n,n+1]</m>, it follows that the union is also closed. I'll leave the details to you.
        </p>
      </li>
      <li>
        <p>
          Let <m>q\colon\R\rightarrow \R/\Z</m> be the quotient map. Consider the diagram
          <image xml:id="eg_quotient_homeo" width="25%">
            <latex-image>
              \begin{tikzcd}
                 \R \arrow[rd, twoheadrightarrow,"g"] \arrow[d, twoheadrightarrow,"q"']\amp \\
                \R/\Z \arrow[r,dotted,"\exists! f"'] \amp S^1
              \end{tikzcd}
            </latex-image>
          </image>
          where <m>g(t)=(\cos 2\pi t, \sin 2\pi t)</m>. It is easy to see that <m>g</m> is continuous, surjective, and satisfies <m>g(t_1)=g(t_2)\iff t_1=t_2+n</m> for some <m>n\in \Z</m>. It follows from <xref ref="cor_quotientspace_props"/> that the map <m>f</m> is bijective and continuous. Furthermore, by the same result, we can show <m>f</m> is a homeomorphism as long as we can show <m>g</m> is a quotient map. I'll show that in fact <m>g\colon \R\rightarrow S^1</m> is open, and hence a projection map.
        </p>
        <p>
        To this end let <m>U\subseteq \R</m> be any open set, and let <m>P\in f(U)</m>, so that <m>P=g(t)</m> for some <m>t\in U</m>. We will find an open interval <m>I</m> satisfying <m>t\in I\subseteq U</m> such that <m>f(I)</m> is open. Since <m>P\in f(I)\subseteq f(U)</m> and <m>P\in f(U)</m> was arbitrary, this will show that <m>f(U)</m> is open.
        </p>
        <p>
          Let <m>g(t)=P=(x,y)</m>. Since we cannot have <m>x=y=0</m>, we have four cases: <m>y&gt;0</m> or <m>y&lt; 0</m> or <m>x&gt; 0</m> or <m>x&lt; 0</m>. I will treat the first case; my argument is easily adapted to the other cases. Assume <m>y&gt; 0</m>. Since the set <m>V=S^1\cap \left(\R\times (0,\infty)\right)</m> is open in <m>S^1</m>, we can find an open interval <m>I=(a,b)\ni t</m> contained in <m>U</m> such <m>g(I)\subseteq V </m>: <ie />, all points in <m>g(I)</m> lie in the the upper half plane. Elementary trigonometric properties tell us that the function <m>h(t)=\cos 2\pi t</m> is strictly decreasing on <m>I</m>, and hence that <m>h(I)</m> is the open interval <m>(\cos 2\pi b, \cos 2\pi a)=(c,d)</m>.
          It is now easy to see that <m>g(I)=\{(x,y)\colon x\in (c,d), y=+\sqrt{1-x^2}\}=S^1\cap \left((c,d)\times \R\right)</m>, which is open.
        </p>
      </li>
    </ol>

  </solution>
</example>

</section>
